# 97. Interleaving String

> Given *s1*, *s2*, *s3*, find whether *s3* is formed by the interleaving of *s1* and *s2*.
>
> **Example 1:**
>
> ```
> Input: s1 = "aabcc", s2 = "dbbca", s3 = "aadbbcbcac"
> Output: true
> ```
>
> **Example 2:**
>
> ```
> Input: s1 = "aabcc", s2 = "dbbca", s3 = "aadbbbaccc"
> Output: false
> ```

动态规划。

代码如下：

```python
class Solution:
    def isInterleave(self, s1: str, s2: str, s3: str) -> bool:
        if s1 == "":
            return s3 == s2
        elif s2 == "":
            return s3 == s1
        elif len(s3) != len(s1) + len(s2):
            return False
        memo = {}
        s1 = list(s1)
        s2 = list(s2)
        s3 = list(s3)
        def dp(i: int, j: int) -> bool:
            k = i + j + 2
            if (i, j) not in memo:
                memo[i, j] = False
                if i == 0:
                    for m in range(k):
                        if s3[m] == s1[0] and s3[0:m] + s3[m+1:k] == s2[0:j+1]:
                            memo[i, j] = True
                            break
                elif j == 0:
                    for m in range(k):
                        if s3[m] == s2[0] and s3[0:m] + s3[m+1:k] == s1[0:i+1]:
                            memo[i, j] = True
                            break
                else:
                    memo[i, j] = (s3[k-1] == s1[i] and dp(i-1, j)) or (s3[k-1] == s2[j] and dp(i, j-1))
            return memo[i, j]
        
        return dp(len(s1)-1, len(s2)-1)
        
```

